>[!question] 3.4.7
Find the general solution of ${x_1' = 3x_1 + x_2, x_2' = 2x_1+4x_2}$, using the eigenvalue method.

>[!check]- Solution
${\vec{x}' = \begin{bmatrix} 3 & 2 \\ 1 & 4 \end{bmatrix}\vec{x}}$
> 
> ${\begin{vmatrix} 3-\lambda & 2 \\ 1 & 4-\lambda \end{vmatrix} = (3-\lambda)(4-\lambda) - 2 = 12 -7\lambda + \lambda^2 - 2 = 10 -7\lambda + \lambda^2}$
> ${(\lambda - 5)(\lambda - 2) = 0}$
> So the eigenvalues are ${\lambda = 5, 2}$
> 
> The eigenvectors are ${\begin{bmatrix} 1 \\ -1\end{bmatrix}, \begin{bmatrix} 1 \\ -2 \end{bmatrix}}$
> 
> ${x = c_1\begin{bmatrix} 1 \\ -1\end{bmatrix}e^{5t} + c_2\begin{bmatrix} 1 \\ -2 \end{bmatrix} e^{2t}}$

3.4.8
Find the general solution of ${x_1' = x_1-2x_2}$, ${x_2' = 2x_1+x_2}$ using the eigenvalue method. Do not use complex exponentials in your solution.

>[!check]- Solution
>${\vec{x}' = \begin{bmatrix} 1 & -2 \\ 2 & 1 \end{bmatrix} x}$
>
>${\begin{vmatrix} 1 - \lambda & -2 \\ 2 & 1-\lambda \end{bmatrix} = (1-\lambda)^2 + 4 = 0}$

3.4.9

3.5.1

3.5.4