**3.2.3**
Compute determinant of ${\begin{bmatrix} 9 & -2 & -6 \\ -8 & 3 & 6 \\ 10 & -2 & -6 \end{bmatrix}}$

${\begin{bmatrix} 9 & -2 & -6 & | & 9 & -2 & -6 \\ -8 & 3 & 6 & | & -8 & 3 & 6 \\ 10 & -2 & -6 & | & 10 & -2 & -6 \end{bmatrix}}$

${\begin{vmatrix} 9 & -2 & -6 \\ -8 & 3 & 6 \\ 10 & -2 & -6 \end{vmatrix} }$

${\begin{align}&= 9 \cdot 3 \cdot (-6) + (-2) \cdot 6 \cdot 10 + (-6) \cdot (-8) \cdot (-2) \\ &- (-6) \cdot 3 \cdot 10 - 6 \cdot (-2) \cdot 9 - (-8) \cdot (-2) \cdot (-6) \end{align}}$

${= -162 - 120 -96 + 180 + 108 + 96 = 6}$


**3.2.6**
For which ${h}$ is ${\begin{bmatrix} 1 & 2 & 3 \\ 4 & 5 & 6 \\ 7 & 8 & h \end{bmatrix}}$ not invertible? Is there only one such ${h}$? Are there several? Infinitely many?

${\begin{bmatrix} 1 & 2 & 3 & | & 0\\ 4 & 5 & 6 & | & 0 \\ 7 & 8 & h & | & 0 \end{bmatrix}}$

${R_2 \rightarrow R_1 \cdot (-4) + R_2}$
${R_3 \rightarrow R_1 \cdot(-7) + R_3}$

${\begin{bmatrix} 1 & 2 & 3 & | & 0\\ 0 & -3 & -6 & | & 0 \\ 0 & -6 & h-21 & | & 0 \end{bmatrix}}$

${R_3 \rightarrow R_2 \cdot (-2) + R_3}$
${R_2 \rightarrow R_2 \cdot (-\frac{1}{3})}$

${\begin{bmatrix} 1 & 2 & 3 & | & 0\\ 0 & 1 & 2 & | & 0 \\ 0 & 0 & h-9 & | & 0 \end{bmatrix}}$

${h - 9 = 0}$
${h = 9}$ is the only solution where the matrix is non-invertible.

**3.3.1**
Write the system ${x_1' = 2x_1 - 3tx_2 + \sin(t)}$, ${x_2' = e^t x_1 + 3x_2 + \cos(t)}$ in the form of ${\vec{x}' = P(t)\vec{x} + \vec{f}(t)}$.

${\vec{x}' = \begin{bmatrix} 2 & -3 \\ e^t & 3 \end{bmatrix}\vec{x} + \begin{bmatrix} \sin(t) \\ \cos(t) \end{bmatrix}}$

**3.3.2**

a) Verify that the system ${\vec{x}' = \begin{bmatrix} 1 & 3 \\ 3 & 1 \end{bmatrix} \vec{x}}$ has the two solutions and ${\begin{bmatrix} 1 \\ 1 \end{bmatrix} e^{4t}}$ and ${\begin{bmatrix} 1 \\ -1 \end{bmatrix} e^{-2t}}$.

${\begin{vmatrix} 1-\lambda & 3 \\ 3 & 1-\lambda \end{vmatrix} = (1-\lambda)^2 - 9 = \lambda^2 - 2\lambda - 8 = (\lambda - 4)(\lambda + 2) = 0}$

${\lambda = 4, -2}$

${\lambda = 4}$
${\begin{bmatrix} 1-4 & 3 & | & 0\\ 3 & 1-4 & | & 0\end{bmatrix} = \begin{bmatrix} -3 & 3 & | & 0\\ 3 & -3 & | & 0\end{bmatrix}}$

${R_2 \rightarrow R_1 \cdot (-1) + R_2}$

${\begin{bmatrix} -3 & 3 & | & 0\\ 0 & 0 & | & 0\end{bmatrix}}$

${R_1 \rightarrow R_1 \cdot (-\frac{1}{3})}$

${\begin{bmatrix} 1 & -1 & | & 0\\ 0 & 0 & | & 0\end{bmatrix}}$

${x_1 = x_2}$

${v_1 = \begin{bmatrix} 1 \\ 1 \end{bmatrix}}$

Solution 1: ${\begin{bmatrix} 1 \\ 1 \end{bmatrix} e^{4t}}$

${\lambda = -2}$
${\begin{bmatrix} 1+2 & 3 & | & 0\\ 3 & 1+2 & | & 0\end{bmatrix} = \begin{bmatrix} 3 & 3 & | & 0\\ 3 & 3 & | & 0\end{bmatrix}}$

${R_2 \rightarrow R_1 \cdot (-1) + R_2}$

${\begin{bmatrix} 3 & 3 & | & 0\\ 0 & 0 & | & 0\end{bmatrix}}$

${R_1 \rightarrow R_1 \cdot \frac{1}{3}}$

${\begin{bmatrix} 1 & 1 & | & 0\\ 0 & 0 & | & 0\end{bmatrix}}$

${x_1 = -x_2}$

${v_2 = \begin{bmatrix} 1 \\ -1 \end{bmatrix}}$

Solution 2: ${\begin{bmatrix} 1 \\ -1 \end{bmatrix} e^{-2t}}$


b) Write down the general solution.

${x = c_1\begin{bmatrix} 1 \\ 1 \end{bmatrix}e^{4t} + c_2\begin{bmatrix} 1 \\ -1 \end{bmatrix}e^{-2t}}$

c) Write down the general solution in the form, (i.e. write down a formula for each element of the solution).

${x_1 = c_1e^{4t} + c_2e^{-2t}}$
${x_2 = c_1e^{4t} - c_2e^{-2t}}$

**3.3.3** Verify that ${\begin{bmatrix} 1 \\ 1\end{bmatrix}e^{t}}$ and ${\begin{bmatrix} 1 \\ -1 \end{bmatrix}e^{t}}$are linearly independent. Hint: Just plug in ${t = 0}$.

If ${t = 0}$

${\begin{bmatrix} 1 \\ 1\end{bmatrix}e^{0} = \begin{bmatrix} 1 \\ 1\end{bmatrix}}$
 
${\begin{bmatrix} 1 \\ -1\end{bmatrix}e^{0} = \begin{bmatrix} 1 \\ -1\end{bmatrix}}$

${c\begin{bmatrix} 1 \\ -1 \end{bmatrix} \neq \begin{bmatrix} 1 \\ 1 \end{bmatrix}}$

for any ${c \in \mathbb{R}}$

So, the two vectors are linearly independent.