>[!question] 6.3.6
>${x(t) = e^{-t} + \int_0^t \cos(t-\tau)x(\tau)d\tau}$

${\mathcal{L}\{x(t)\} = \mathcal{L}\{e^{-t}\} + \mathcal{L}\{\cos(t) * x(t)\}}$

${X(s) = \frac{1}{s+1} + \mathcal{L}\{\cos(t)\} \mathcal{L}\{x(t)\}}$

${\implies X(s) = \frac{1}{s+1} + \frac{s}{s^2+1} X(s)}$
${\implies (1-\frac{s}{s^2+1})X(s) = \frac{1}{s+1}}$
${\frac{s^2-s+1}{s^2+1}X(s) = \frac{1}{s+1}}$
${\implies X(s) = \frac{s^2+1}{(s+1)(s^2-s+1)}}$

Partial Fractions

${s^2+1 = (As+B)(s+1) + C(s^2-s+1)}$
if ${s = -1}$
${1 + 1 = 3C}$
${C = \frac{2}{3}}$
Compare coefficients
${As^2 + \frac{2}{3}s^2  = s^2}$
${A + \frac{2}{3} = 1}$
${A = \frac{1}{3}}$
${1 = B + \frac{2}{3}}$
${B = \frac{1}{3}}$

${X(s) = \dfrac{\frac{1}{3}s + \frac{1}{3}}{s^2-s+1} + \dfrac{\frac{2}{3}}{s+1} = \dfrac{\frac{1}{3}s + \frac{1}{3}}{(s-0.5)^2 + \frac{3}{4}} + \dfrac{\frac{2}{3}}{s+1}}$
${= \frac{1}{3} \left(\dfrac{s+1}{(s-0.5)^2 + \frac{3}{4}} + \dfrac{2}{s+1}\right)}$ 
${= \frac{1}{3} \left(\dfrac{s-0.5}{(s-0.5)^2 + \frac{3}{4}} + \dfrac{2}{s+1} \right) + \dfrac{0.5}{(s-0.5^2) + \frac{3}{4}}}$
${= \frac{2}{3}e^{-t} + \frac{1}{3}e^{0.5t}\cos(\frac{\sqrt{3}}{2}) + \frac{1}{\sqrt{3}}e^{0.5t}\sin(\frac{\sqrt{3}}{2}t)}$

>[!question] 6.4.6
>Compute ${\mathcal{L}^{-1}\left\{\frac{s^2+s+1}{s^2}\right\}}$

${\mathcal{L^{-1}}\{1\} + \mathcal{L}^{-1}\{\frac{1}{s}\} + \mathcal{L}^{-1}\{\frac{1}{s^2}\}}$

${\delta(t) + 1 + t}$

>[!question] 3.1.2
>${x_1' = x_2 - x_1 + t, x_2' = x_2}$

${x_1'' = Ce^t - x_1' + 1}$
${x_1'' + x_1' = Ce^t + 1}$
${\mu = e^{\int 1dt} = e^t}$

${x_1' = \dfrac{\int e^{t}(Ce^{t}+1)dt + C_2}{e^{t}} = \dfrac{\int Ce^{2t} + e^{t} dt}{e^{t}} = \frac{C} {2}e^{2t} + e^{t} + C_2{e^t} = \frac{C}{2}e^{t} + 1 + C_2e^{-t}}$

${x_1 = \int x_1' dt = \frac{C}{2}e^t + t  -C_2e^{-t}}$

>[!question] 3.1.5
Write ${x'' + y^2y' - x^3 = \sin(t), y'' + (x' + y')^2 - x = 0}$ as a first order system of ODEs.

${x_1 = x, x_2 = x', x_3 = y, x_4 = y'}$

${x_1' = x_2}$
${x_2' = \sin(t) + x_1^3 - x_2^2x_4}$
${x_3' = x_4}$
${x_4' = x_1 - (x_2 + x_4)^2}$

>[!question] 3.2.10
>Solve ${\begin{bmatrix} 3 & 2 & 3 & 0 \\ 3 & 3 & 3 & 3 \\ 0 & 2 & 4 & 2 \\ 2 & 3 & 4 & 3 \end{bmatrix}\vec{x} = \begin{bmatrix} 2 \\ 0 \\ 4 \\ 1\end{bmatrix}}$

${\begin{bmatrix} 3 & 2 & 3 & 0 & | & 2\\ 3 & 3 & 3 & 3 & | & 0\\ 0 & 2 & 4 & 2 & | & 4\\ 2 & 3 & 4 & 3 & | & 1\end{bmatrix}}$

${R_1 \cdot (-1) + R_2 }$
${R_1 \cdot (-\frac{2}{3}) + R_4}$

${\begin{bmatrix} 3 & 2 & 3 & 0 & | & 2\\ 0 & 1 & 0 & 3 & | & -2\\ 0 & 2 & 4 & 2 & | & 4\\ 0 & \frac{5}{3} & 2 & 3 & | & -\frac{1}{3}\end{bmatrix}}$

${R_1 \cdot \frac{1}{3}}$
${R_2 \cdot (-2) + R_3}$
${R_2 \cdot (-\frac{5}{3}) + R_4}$

${\begin{bmatrix} 1 & \frac{2}{3} & 1 & 0 & | & \frac{2}{3}\\ 0 & 1 & 0 & 3 & | & -2\\ 0 & 0 & 4 & -4 & | & 8 \\ 0 & 0 & 2 & -2 & | & 3\end{bmatrix}}$

${R_3 \cdot \frac{1}{4}}$

${\begin{bmatrix} 1 & \frac{2}{3} & 1 & 0 & | & \frac{2}{3}\\ 0 & 1 & 0 & 3 & | & -2\\ 0 & 0 & 1 & -1 & | & 2 \\ 0 & 0 & 2 & -2 & | & 3\end{bmatrix}}$

${R_3 \cdot -2 + R_4}$

${\begin{bmatrix} 1 & \frac{2}{3} & 1 & 0 & | & \frac{2}{3}\\ 0 & 1 & 0 & 3 & | & -2\\ 0 & 0 & 1 & -1 & | & 2 \\ 0 & 0 & 0 & 0 & | & -1\end{bmatrix}}$

No solution, ${0 = -1}$

