1. Define alphabet $\Sigma = \{0,1\}$. Write a regular expression for all strings on $\Sigma$ with at least two $1$'s.

$(0+1)^*(1)(0+1)^*(1)(0+1)^*$


2. Write a regular expression for all strings on $\Sigma$ with exactly two $1$'s.

$(0)^*(1)(0)^*(1)(0)^*$

3. Write a regular expression for all strings on $\Sigma$ containing substrings $101$ and $010$.

Case 1: $(0+1)^* (101)(0+1)^*(010) (0+1)^*$
Case 2: $(0+1)^* (010)(0+1)^*(101) (0+1)^*$
Case 3: $(0+1)^* (1010) (0+1)^*$
Case 4: $(0+1)^* (0101) (0+1)^*$

Don't try to simplify

4. All strings on the alphabet $\Sigma$ that do not end with $111$

Case 1: End with $0$
Case 2: End with $01$
Case 3: End with $011$
Case 4: Short strings
e.g. empty, $1$, $11$

$(0+1)^*0 + (0+1)^*01+(0+1)^*011 + \Lambda + 1 + 11$

5. All strings that do not have $111$ as substring

Note: concept of "substring"
$$abababa$$

6. Proof Writing

> **Theorem** $$(L_1+L_2)^* = (L_1^* + L_2^*)^*$$

1. $$(L_1+L_2)^* \subseteq (L_1^* + L_2^*)^*$$

Note $L_1 \subseteq L_1^*$ and $L_2 \subseteq L_2^*$ so the above must hold.

2. $$(L_1^*+L_2^*)^* \subseteq (L_1+L_2)^*$$

$$(L_1^* + L_2^*)^* = \bigcup_{k\ge 0}(L_1^*+L_2^*)^k = \bigcup_{k\ge0}\bigcup_{i_1,...,i_k \in \{1,2\}}(L_{i_1}^*...L_{i_k}^*)^k$$
$$\subseteq \bigcup_{k \ge 0}\bigcup_{i_1,...,i_k \in \{1,2\}}(L_1+L_2)^*...(L_1+L_2)^* = \bigcup_{k \ge 0}\bigcup_{i_1,...,i_k \in \{1,2\}}(L_1+L_2)^*$$


> **Lemma** Show $L^*L^* = L^*$

*Proof:*
$L^*L^* = \bigcup_{k\ge 0}L^k \bigcup_{m\ge0}(L^m) = \bigcup_{k,m\ge0}L^k\cdot L^m$

$= \bigcup_{k,m \ge 0} L^{k+m} = \bigcup_{n\ge0}L^n = L^*$

> **Theorem** Using structured induction to prove:
$Appear(L,b) = \{x: x\in L \text{ and }x \text{ contains symbol b}\}$ is regular
if $L$ is.

*Proof:*
Use structural induction according to definition of regular languages.
1. $L = \emptyset$ is regular. $Appear(L,b) = Appear(\emptyset, b) = \emptyset$ which is regular
2. $L = \{\wedge\}$ is regular. $Appear(L,b) = Appear(\wedge, b) = \emptyset$ which is regular
3. $L= \{a\}$, $a \in \Sigma$ is regular $Appear(L,b) = Appear(a,b) = \begin{cases} \{b\} & \text{if }a=b \\ \emptyset & \text{if }a\neq b \end{cases}$
4. If $L_1$ and $L_2$ are regular, so are
	1.  $L_1+L_2$
	2. $L_1L_2$
	3. $L_1^*$

$Appear(L_1,b)$ and $Appear(L_2,b)$ are regular,
$Appear(L_1+L_2,b)$
Take $L = L_1 + L_2$ which is regular
$Appear(L,b) = Appear(L_1,b) \cup Appear(L_2,b)$ which is regular
$Appear(L_1L_2,b) = L_1Appear(L_2,b) + Appear(L_1,b)L_2$
$Appear(L_1^*)$ $= Appear(L_1^0 \cup L_1^1 ...,b) = Appear(L_1,b) \cup Appear(L_2,b)...$
Union of regular is regular

___

Sketch an algorithm to find shortest odd-length words in a regular expression.

___

Use Pumping Lemma to show $L = \{a^nb^n : n > 0\}$ is not regular